a better spec of dft_[br,std] and bft_[br_std]

bft_spec.v
@@ -13,174 +13,17 @@ Require Import utils bt bft.
 
 Set Implicit Arguments.
 
-Section map.
-
-  Variables (X Y : Type) (f g : X -> Y).
-
-  Fact map_ext l : (forall x, In x l -> f x = g x) -> map f l = map g l.
-  Proof. rewrite <- Forall_forall; induction 1; simpl; f_equal; auto. Qed.
-
-End map.
-
-Section map_concat_zip.
-
-  Variable (X Y : Type) (f : X -> Y) (g : X -> X -> X) (h : Y -> Y -> Y).
-
-  Fact map_concat ll : map f (concat ll) = concat (map (map f) ll).
-  Proof. 
-    induction ll; simpl; f_equal; auto.
-    rewrite map_app; f_equal; auto.
-  Qed.
-
-  Hypothesis Hgh : forall x y, f (g x y) = h (f x) (f y). 
-
-  Fact map_zip l m : map f (zip g l m) = zip h (map f l) (map f m).
-  Proof. revert m; induction l; intros [|]; simpl; f_equal; auto. Qed.
-
-End map_concat_zip.
-
-Section zip_app.
-
-  Variable (X : Type).
-
-(*
-  Fact zip_app_left l m x u : In x u -> In u l -> In x (zip (@app X) l m).
-  Proof.
-    revert m; induction l as [ | y l IHl ]; intros [|]; simpl; try tauto.
-    intros [|]; subst.
-*)
-End zip_app.
-
-Section sorted.
-
-  Variable (X : Type) (R : X -> X -> Prop).
-
-  Inductive sorted : list X -> Prop :=
-    | in_sorted_0 : sorted nil
-    | in_sorted_1 : forall x l, Forall (R x) l -> sorted l -> sorted (x::l).
-
-  Fact sorted_app l m : (forall x y, In x l -> In y m -> R x y) -> sorted l -> sorted m -> sorted (l++m).
-  Proof.
-    intros H H1 Hm; revert H1 H.
-    induction 1 as [ | x l H1 H2 IH2 ]; intros H3; simpl; auto.
-    constructor.
-    + apply Forall_app; auto.
-      apply Forall_forall; intros; apply H3; simpl; auto.
-    + apply IH2; intros; apply H3; simpl; auto.
-  Qed.
-
-  Variable (f : X -> X) (Hf : forall x y, R x y -> R (f x) (f y)).
-
-  Fact sorted_map l : sorted l -> sorted (map f l).
-  Proof.
-    induction 1 as [ | x l H1 H2 IH2 ]; simpl; constructor; auto.
-    apply Forall_forall.
-    rewrite Forall_forall in H1.
-    intros y; rewrite in_map_iff.
-    intros (? & ? & ?); subst; auto.
-  Qed.
-
-End sorted.
-
-Fact sorted_mono X (R S : X -> X -> Prop) l : (forall x y, In x l -> In y l -> R x y -> S x y) -> sorted R l -> sorted S l.
-Proof.
-  intros H1 H2; revert H2 H1.
-  induction 1 as [ | x l H1 H2 IH2 ]; intros H3.
-  + constructor.
-  + constructor.
-    * revert H1; do 2 rewrite Forall_forall.
-      intros H1 y Hy; apply H3; simpl; auto.
-    * apply IH2; intros ? ? ? ?; apply H3; simpl; auto.
-Qed.
-
-Section increase.
- 
-  Variable (X : Type) (P : nat -> X -> Prop).
-
-  Inductive increase : nat -> list X -> Prop :=
-    | in_increase_0 : forall n, increase n nil
-    | in_increase_1 : forall n x l, P n x -> increase (S n) l -> increase n (x::l).
-
-  Fact increase_inv n l x : increase n l -> In x l -> exists k, n <= k /\ P k x.
-  Proof.
-    intros H Hx; revert H; induction 1 as [ n | n y l H1 H2 IH2 ]; simpl.
-    + destruct Hx.
-    + destruct Hx as [ | Hx ]; subst.
-      * exists n; split; auto.
-      * destruct IH2 as (k & ? & ?); auto.
-        exists k; split; auto; omega.
-  Qed.
-
-  Section zip.
-
-     Variable (f : X -> X -> X) (Hf : forall n x y, P n x -> P n y -> P n (f x y)).
-
-     Fact zip_increase l m n : increase n l -> increase n m -> increase n (zip f l m).
-     Proof.
-       intros H; revert H m.
-       induction 1 as [ n | n x l H1 H2 IH2 ]; simpl; intros m Hm; auto.
-       destruct m as [ | y m ]; simpl.
-       * constructor; auto.
-       * constructor; inversion Hm; auto.
-     Qed.
-
-  End zip.
-
-  Section map.
-
-    Variable (f : X -> X) (Hf : forall n x, P n x -> P (S n) (f x)).
-
-    Fact map_increase n l : increase n l -> increase (S n) (map f l).
-    Proof. induction 1; simpl; constructor; auto. Qed.
-
-  End map.
-
-End increase.
-
-Section sorted_concat.
-
-  Variable (X : Type) (P : nat -> list X -> Prop) (R : X -> X -> Prop) 
-           (HPR : forall i j x l y m, i < j -> P i l -> P j m -> In x l -> In y m -> R x y).
-
-  Fact concat_sorted n ll : increase P n ll -> Forall (sorted R) ll -> sorted R (concat ll).
-  Proof.
-    induction 1 as [ n | n l ll H1 H2 IH2 ]; simpl.
-    + constructor.
-    + inversion 1; subst.
-      apply sorted_app; auto.
-      intros x y; rewrite in_concat_iff.
-      intros G1 (m & G2 & G3).
-      apply increase_inv with (2 := G3) in H2.
-      destruct H2 as (k & H0 & H2).
-      revert G1 G2; apply (@HPR n k); auto.
-  Qed.
-
-End sorted_concat.
-
 Section bt_branches.
 
   Variable X : Type.
 
-  Unset Elimination Schemes.
-
-  Inductive btb : list bool -> bt X -> Prop :=
-    | in_btb_0 : forall t, btb nil t
-    | in_btb_1 : forall l u x v, btb l u -> btb (false::l) (node u x v)
-    | in_btb_2 : forall l u x v, btb l v -> btb (true::l)  (node u x v).
-
-  Set Elimination Schemes.
-
-  Scheme btb_ind := Induction for btb Sort Prop.
-
-  Hint Constructors btb.
-
-  Fact btb_inv_1 l u x v : btb (false::l) (node u x v) -> btb l u.
-  Proof. inversion 1; trivial. Defined.
-
-  Fact btb_inv_2 l u x v : btb (true::l) (node u x v) -> btb l v.
-  Proof. inversion 1; trivial. Defined.
-
   (* The tree branches by Depth First Traversal *)
+
+  Fixpoint dft_std (t : bt X) :=
+    match t with 
+      | leaf x => x::nil
+      | node u x v => x::dft_std u++dft_std v
+    end.
 
   Fixpoint dft_br (t : bt X) : list (list bool) :=
     nil::match t with 
@@ -190,7 +33,7 @@ Section bt_branches.
 
   (* branches t included in btb _ t *)
 
-  Fact dft_br_spec_1 t : Forall (fun l => btb l t) (dft_br t).
+  Fact dft_br_spec_1 t : Forall (btb t) (dft_br t).
   Proof.
     induction t as [ x | u Hu x v Hv ].
     + do 2 constructor.
@@ -202,7 +45,7 @@ Section bt_branches.
 
   (* dft_br contains the branches of t *)
 
-  Fact dft_br_spec l t : btb l t <-> In l (dft_br t).
+  Fact dft_br_spec l t : btb t l <-> In l (dft_br t).
   Proof.
     split.
     + induction 1 as [ t | l u x v H IH | m u x v H IH ]; simpl.
@@ -216,40 +59,6 @@ Section bt_branches.
 
   Fact dft_br_spec_2 t : length (dft_br t) = m_bt t.
   Proof. induction t; simpl; auto; rewrite app_length; repeat rewrite map_length; omega. Qed.
-
-  Inductive lb_lex : list bool -> list bool -> Prop :=
-    | in_lb_0 : forall l, lb_lex nil l
-    | in_lb_1 : forall l m, lb_lex (false::l) (true::m)
-    | in_lb_2 : forall b l m, lb_lex l m -> lb_lex (b::l) (b::m).
-
-  Fact lb_lex_refl l : lb_lex l l.
-  Proof. induction l; constructor; auto. Qed.
-
-  Fact lb_lex_trans l m k : lb_lex l m -> lb_lex m k -> lb_lex l k.
-  Proof.
-    intros H; revert H k.
-    induction 1 as [ l | l m | b l m H IH ]; intros k H1.
-    + constructor.
-    + inversion H1; constructor.
-    + inversion H1; constructor; auto.
-  Qed.
-
-  Fact lb_lex_antisym l m : lb_lex l m -> lb_lex m l -> l = m.
-  Proof. induction 1; inversion 1; f_equal; auto. Qed.
-
-  Definition lb_lex_dec l m : { lb_lex l m } + { lb_lex m l }.
-  Proof.
-    revert m; induction l as [ | [] l IHl ]; intros m.
-    + left; constructor.
-    + destruct m as [ | [] m ].
-      * right; constructor.
-      * destruct (IHl m); [ left | right ]; constructor; auto.
-      * right; constructor.
-    + destruct m as [ | [] m ].
-      * right; constructor.
-      * left; constructor.
-      * destruct (IHl m); [ left | right ]; constructor; auto.
-  Qed.
 
   (* the branches of t in dft_br t are sorted according to lb_lex *)
 
@@ -266,35 +75,13 @@ Section bt_branches.
         - apply sorted_map; auto; constructor; auto.
   Qed.
 
-  (* The Breadth First Search order between bt branches *)
+  (* dft_br corresponds to dft_std *)
 
-  Definition bft_order l m := length l < length m \/ length l = length m /\ lb_lex l m.
-
-  Fact bft_order_refl l : bft_order l l.
-  Proof. right; split; auto; apply lb_lex_refl. Qed.
-
-  Fact bft_order_antisym l m :  bft_order l m ->  bft_order m l -> l = m.
+  Fact dft_br_spec_4 t : Forall2 (bt_path_node t) (dft_br t) (dft_std t).
   Proof.
-    intros [ | [] ] [ | [] ]; try omega.
-    apply lb_lex_antisym; auto.
-  Qed.
-
-  Fact bft_order_trans l m k : bft_order l m -> bft_order m k -> bft_order l k.
-  Proof.
-    intros [ | [] ] [ | [] ]; try (left; omega).
-    right; split; try omega.
-    apply lb_lex_trans with m; auto.
-  Qed.
- 
-  Definition bft_order_dec l m : { bft_order l m } + { bft_order m l }.
-  Proof.
-    destruct (le_lt_dec (length l) (length m)).
-    2: right; left; auto.
-    destruct (le_lt_dec (length m) (length l)).
-    2: left; left; auto.
-    destruct (lb_lex_dec l m).
-    * left; right; split; auto; omega.
-    * right; right; split; auto; omega.
+    induction t as [ x | u Hu x v Hv ]; simpl; repeat constructor.
+    apply Forall2_app; apply Forall2_map_left; [ revert Hu | revert Hv ];
+      apply Forall2_mono; constructor; auto.
   Qed.
 
   Fixpoint niveaux_br (t : bt X) : list (list (list bool)) :=
@@ -304,7 +91,7 @@ Section bt_branches.
                                                  (map (map (cons true))  (niveaux_br b))
     end.
 
-  Fact niveaux_br_spec_1 t : forall l ll, In l ll -> In ll (niveaux_br t) -> btb l t.
+  Fact niveaux_br_spec_1 t : forall l ll, In l ll -> In ll (niveaux_br t) -> btb t l.
   Proof.
     induction t as [ x | u Hu x v Hv ]; simpl; intros l ll H1 H2.
     * destruct H2 as [ | [] ]; subst.
@@ -336,7 +123,7 @@ Section bt_branches.
           ** constructor; apply Hv with (2 := H4); auto.
   Qed.
 
-  Fact niveaux_br_spec_0 l t : btb l t -> exists ll, In l ll /\ In ll (niveaux_br t).
+  Fact niveaux_br_spec_0 l t : btb t l -> exists ll, In l ll /\ In ll (niveaux_br t).
   Proof.
     induction 1 as [ t | l u x v H (ll & H1 & H2) | m u x v H (mm & H1 & H2) ].
     + exists (nil::nil); destruct t; simpl; auto.
@@ -388,7 +175,7 @@ Section bt_branches.
           ++ apply in_map; simpl; auto.
   Qed.
 
-  Fact niveaux_br_spec l t : btb l t <-> exists ll, In l ll /\ In ll (niveaux_br t).
+  Fact niveaux_br_spec l t : btb t l <-> exists ll, In l ll /\ In ll (niveaux_br t).
   Proof.
     split.
     + apply niveaux_br_spec_0.
@@ -440,7 +227,7 @@ Section bt_branches.
 
   (* bft_br contains the branches of t *)
 
-  Fact bft_br_spec_1 l t : In l (bft_br t) <-> btb l t.
+  Fact bft_br_spec_1 l t : In l (bft_br t) <-> btb t l.
   Proof. unfold bft_br; rewrite niveaux_br_spec, in_concat_iff; tauto. Qed.
  
   Hint Resolve niveaux_br_spec_2.
@@ -526,7 +313,19 @@ Section bt_branches.
     rewrite map_zip with (h := @app _).
     2: intros; apply map_app.
     rewrite Hu, Hv; repeat rewrite map_map; f_equal;
-    apply map_ext; intros l _; rewrite map_map; apply map_ext; intros; simpl; auto.
+    apply map_ext; intros; rewrite map_map; apply map_ext; intros; simpl; auto.
+  Qed.
+
+  Fact niveaux_br_spec_5 t : Forall2 (Forall2 (bt_path_node t)) (niveaux_br t) (niveaux_tree t).
+  Proof.
+    induction t as [ x | u Hu x v Hv ]; simpl; repeat constructor.
+    apply Forall2_zip_app; apply Forall2_map_left.
+    + revert Hu; apply Forall2_mono.
+      intros ? ? H; apply Forall2_map_left; revert H.
+      apply Forall2_mono; constructor; auto.
+    + revert Hv; apply Forall2_mono.
+      intros ? ? H; apply Forall2_map_left; revert H.
+      apply Forall2_mono; constructor; auto.
   Qed.
 
   (* The list of nodes computed by bft_std is the direct map of the sorted list of branches,
@@ -535,11 +334,17 @@ Section bt_branches.
   Theorem bft_br_spec_3 t : map (@Some _) (bft_std t) = map (fun l => btb_node l t) (bft_br t).
   Proof. unfold bft_std, bft_br; rewrite map_concat, map_concat, niveaux_br_spec_4; auto. Qed.
 
+  (* bft_br corresponds to bft_std *)
+
+  Theorem bft_br_spec_4 t : Forall2 (bt_path_node t) (bft_br t) (bft_std t).
+  Proof. apply Forall2_concat, niveaux_br_spec_5. Qed.
+ 
 End bt_branches.
 
 Check dft_br_spec.
 Check dft_br_spec_3.
+Check dft_br_spec_4.
 
 Check bft_br_spec_1.
 Check bft_br_spec_2.
-Check bft_br_spec_3.
+Check bft_br_spec_4.
