bt.v
@@ -9,7 +9,7 @@
 
 (** Binary trees *)
 
-Require Import List.
+Require Import Arith Omega List.
 
 Set Implicit Arguments.
 
@@ -31,10 +31,127 @@ Section bt.
       | node a _ b => 1 + m_bt a + m_bt b
     end.
 
+  Unset Elimination Schemes.
+
+  Inductive btb : bt -> list bool -> Prop :=
+    | in_btb_0 : forall t, btb t nil
+    | in_btb_1 : forall l u x v, btb u l -> btb (node u x v) (false::l) 
+    | in_btb_2 : forall l u x v, btb v l -> btb (node u x v) (true::l).
+
+  Set Elimination Schemes.
+
+  Scheme btb_ind := Induction for btb Sort Prop.
+
+  Hint Constructors btb.
+
+  Fact btb_inv_1 l u x v : btb (node u x v) (false::l) -> btb u l.
+  Proof. inversion 1; trivial. Defined.
+
+  Fact btb_inv_2 l u x v : btb (node u x v) (true::l) -> btb v l.
+  Proof. inversion 1; trivial. Defined.
+
+  Inductive bt_path_node : bt -> list bool -> X -> Prop :=
+    | in_bpn_0 : forall t, bt_path_node t nil (root t)
+    | in_bpn_1 : forall l u x v r, bt_path_node u l r -> bt_path_node (node u x v) (false::l) r
+    | in_bpn_2 : forall l u x v r, bt_path_node v l r -> bt_path_node (node u x v) (true::l) r.
+
+  Fact btb_spec l t : btb t l <-> exists x, bt_path_node t l x.
+  Proof.
+    split.
+    + induction 1 as [ t | l u x v _ (y & Hy) | l u x v _ (y & Hy) ].
+      * exists (root t); constructor.
+      * exists y; constructor; auto.
+      * exists y; constructor; auto.
+    + intros (r & H); revert H.
+      induction 1; constructor; auto.
+  Qed.
+
 End bt.
 
 Arguments root {X}.
 Arguments m_bt {X}.
+
+Hint Constructors btb.
+
+Section branch_orders.
+
+  Reserved Notation "x '<l' y" (at level 70, no associativity).
+  Reserved Notation "x '<b' y" (at level 70, no associativity).
+
+  (* The Depth First Traversal order between bt branches *)
+
+  Inductive lb_lex : list bool -> list bool -> Prop :=
+    | in_lb_0 : forall b l, nil <l b::l
+    | in_lb_1 : forall l m, false::l <l true::m
+    | in_lb_2 : forall b l m, l <l m -> b::l <l b::m
+  where "x <l y" := (lb_lex x y).
+
+  Fact lb_lex_irrefl l : ~ l <l l.
+  Proof. 
+    assert (forall l m, l <l m -> l <> m) as H.
+    { induction 1; try discriminate; inversion 1; tauto. }
+    intros H1; apply (H _ _ H1); auto.
+  Qed.
+
+  Fact lb_lex_trans l m k : l <l m -> m <l k -> l <l k.
+  Proof.
+    intros H; revert H k.
+    induction 1; inversion 1; constructor; auto.
+  Qed. 
+
+  Definition lb_lex_dec l m : { l <l m } + { l = m } + { m <l l }.
+  Proof.
+    revert m; induction l as [ | [] l IHl ]; intros [ | [] m ].
+    + tauto.
+    + do 2 left; constructor.
+    + do 2 left; constructor.
+    + right; constructor.
+    + destruct (IHl m) as [ [ ? | ? ] | ? ].
+      * do 2 left; constructor; auto.
+      * subst; left; right; auto.
+      * right; constructor; auto.  
+    + right; constructor.
+    + right; constructor.
+    + do 2 left; constructor.
+    + destruct (IHl m) as [ [ ? | ? ] | ? ].
+      * do 2 left; constructor; auto.
+      * subst; left; right; auto.
+      * right; constructor; auto.
+   Qed.
+
+  (* The Breadth First Traversal order between bt branches *)
+
+  Definition bft_order l m := length l < length m \/ length l = length m /\ l <l m.
+
+  Notation "l <b m" := (bft_order l m).
+
+  Fact bft_order_irrefl l : ~ l <b l.
+  Proof. 
+    intros [ H | (_ & H) ]; revert H.
+    + apply lt_irrefl.
+    + apply lb_lex_irrefl.
+  Qed.
+
+  Fact bft_order_trans l m k : l <b m -> m <b k -> l <b k.
+  Proof.
+    intros [ | [] ] [ | [] ]; try (left; omega).
+    right; split; try omega.
+    apply lb_lex_trans with m; auto.
+  Qed.
+ 
+  Definition bft_order_dec l m : { l <b m } + { l = m } + { m <b l }.
+  Proof.
+    destruct (le_lt_dec (length l) (length m)).
+    2: right; left; auto.
+    destruct (le_lt_dec (length m) (length l)).
+    2: do 3 left; auto.
+    destruct (lb_lex_dec l m) as [[|]|].
+    + do 2 left; right; split; auto; omega.
+    + tauto.
+    + do 2 right; split; auto; omega.
+  Qed.
+
+End branch_orders.
 
 Reserved Notation "x '~t' y" (at level 70, no associativity).
 Reserved Notation "x '~lt' y" (at level 70, no associativity).
@@ -59,3 +176,5 @@ Notation "x ~t y" := (bt_eq x y).
 Notation "l ~lt m" := (Forall2 bt_eq l m).
 
 Hint Constructors bt_eq.
+
+
